timing/examples/x86_wcet_comparison/rvs_x86_wcet_comparison/annotations-timing/rvs_analysis.c
@@ -1,2 +1,1 @@
 /* loop_max_iter */
-#pragma RVS ["collatz@L1"] loop_max_iter("100")
