timing/examples/FreeRTOS/list/vListInsert.v
@@ -25,7 +25,7 @@ Import Program_vListInsert vListInsert.
 Module p <: LinkedListParams.
   Definition w := 32.
   Definition e := LittleE.
-  Definition dw := 8.
+  Definition dw := 4.
   Definition pw := 4.
   Global Transparent w e dw pw.
 End p.
@@ -68,32 +68,35 @@ Definition insertion_index mem l le_node le_dist le_val new_val len :=
         ((d <= le_dist)%nat <-> v <= new_val).
 
 Definition vListInsert_timing_invs (base_mem : memory)
-    (pxList pxNewListItem le_node sentry : addr) 
+    (pxList pxListHead pxNewListItem le_node sentry : addr) 
     (new_val le_val : N)
     (le_dist len : nat) (t:trace) : option Prop :=
 match t with (Addr a, s) :: t' => match a with
 | 0x800023f0 => Some (
-    insertion_index base_mem pxList le_node le_dist le_val new_val len /\
-    node_distance (s V_MEM32) pxList sentry (len - 1) /\
+    insertion_index base_mem pxListHead le_node le_dist le_val new_val len /\
+    node_distance (s V_MEM32) pxListHead sentry (len - 1) /\
     list_node_value (s V_MEM32) sentry = Some portMAX_DELAY /\
+    list_node_next (s V_MEM32) sentry = Some pxListHead /\
     s R_A0 = pxList /\ s R_A1 = pxNewListItem /\ s V_MEM32 = base_mem /\
     s V_MEM32 Ⓓ[pxNewListItem] = new_val /\
-    pxList <> NULL /\ len <> 0%nat /\
-    node_distance base_mem pxList NULL len /\
+    pxList ⊕ 8 = sentry /\
+    pxListHead <> NULL /\ len <> 0%nat /\
+    sentry <> NULL /\
     cycle_count_of_trace t' = 0
   )
-| 0x8000242c => Some (exists ctr,
-    insertion_index base_mem pxList le_node le_dist le_val new_val len /\
-    node_distance (s V_MEM32) pxList sentry (len - 1) /\
+| 0x8000242c => Some (exists ctr nxt,
+    insertion_index base_mem pxListHead le_node le_dist le_val new_val len /\
+    node_distance (s V_MEM32) pxListHead sentry (len - 1) /\
     list_node_value (s V_MEM32) sentry = Some portMAX_DELAY /\
     (base_mem Ⓓ[pxNewListItem] =? portMAX_DELAY) = false /\
-    s R_A0 <> NULL /\
-    pxList <> NULL /\ s V_MEM32 = base_mem /\
+    (* s R_A4 <> NULL /\ *)
+    pxListHead <> NULL /\ s V_MEM32 = base_mem /\
     s R_A1 = pxNewListItem /\ s R_A3 = new_val /\
     len <> 0%nat /\
     (ctr <= le_dist)%nat /\
-    node_distance base_mem pxList NULL len /\
-    node_distance base_mem pxList (s R_A0) ctr /\
+    list_node_next (s V_MEM32) (s R_A4) = Some nxt /\
+    node_distance base_mem pxListHead nxt ctr /\
+    sentry <> NULL /\
     cycle_count_of_trace t' =
       tlw + taddi + taddi +
       ttbne + (N.of_nat ctr) * (
@@ -163,8 +166,12 @@ Proof.
         now symmetry.
 Qed.
 
+Lemma Some_inv : forall (X : Type) (x y : X),
+    Some x = Some y -> x = y.
+Proof. intros. now inversion H. Qed.
+
 Theorem vListInsert_timing:
-  forall s t s' x' base_mem len pxList pxNewListItem le_node le_dist le_val sentry new_val
+  forall s t s' x' base_mem len pxList pxListHead pxNewListItem le_node le_dist le_val sentry new_val
          (* boilerplate *)
          (ENTRY: startof t (x',s') = (Addr entry_addr, s))
          (MDL: models rvtypctx s)
@@ -174,18 +181,20 @@ Theorem vListInsert_timing:
          (A1: s R_A1 = pxNewListItem)
          (* contents of pxNewListItem *)
          (VAL: s V_MEM32 Ⓓ[pxNewListItem] = new_val)
-         (* list length is finite *)
-         (LEN: node_distance (s V_MEM32) pxList NULL len)
-         (* pxList is non-null *)
-         (L_NN: pxList <> NULL)
+         (* pxListHead is non-null *)
+         (L_NN: pxListHead <> NULL)
+         (LEN: (0 < len)%nat)
          (* there is a sentry node *)
-         (SENTRY: node_distance (s V_MEM32) pxList sentry (len - 1))
+         (HD: 8 ⊕ pxList = sentry)
+         (SENTRY: node_distance (s V_MEM32) pxListHead sentry (len - 1))
          (SENTRY_VAL: list_node_value (s V_MEM32) sentry = Some portMAX_DELAY)
+         (SENTRY_NEXT: list_node_next (s V_MEM32) sentry = Some pxListHead)
+         (SENTRY_NN: sentry <> NULL)
          (* there is an index to insert at *)
-         (IDX: insertion_index base_mem pxList le_node le_dist le_val new_val len),
+         (IDX: insertion_index base_mem pxListHead le_node le_dist le_val new_val len),
   satisfies_all
     lifted_prog
-    (vListInsert_timing_invs base_mem pxList pxNewListItem le_node sentry new_val le_val le_dist len)
+    (vListInsert_timing_invs base_mem pxList pxListHead pxNewListItem le_node sentry new_val le_val le_dist len)
     exits
   ((x',s')::t).
 Proof using.
@@ -194,9 +203,7 @@ Proof using.
 
     Local Ltac step := tstep r5_step.
     simpl. rewrite ENTRY. unfold entry_addr. repeat step.
-    split. assumption. repeat split; auto.
-    eapply head_nonnull_impl_len_nonzero; eassumption.
-    now rewrite <- MEM.
+    split. assumption. repeat split; auto. lia.
 
     intros.
     eapply startof_prefix in ENTRY; try eassumption.
@@ -206,75 +213,66 @@ Proof using.
 
     destruct_inv 32 PRE.
 
-    - destruct PRE as (IDX & SENTRY & SENTRY_VAL & A0 & A1 & MEM & NewVal & NonNull & L_NN & Len_Nz & Cycles).
+    - destruct PRE as (IDX & SENTRY & SENTRY_VAL & SENTRY_NEXT & A0 & A1 & MEM & 
+        NewVal & PXLH & NonNull & Len_Nz & SENTRY_NN & Cycles).
         do 4 step.
-        -- exists 0%nat. split. assumption.
+        -- exists 0%nat, pxListHead. split. assumption.
             repeat split; auto; try now rewrite <- MEM.
             unfold portMAX_DELAY. lia. lia.
+            rewrite N.add_comm, PXLH, <- MEM. assumption.
             apply Dst0.
             hammer.
         -- repeat step. unfold portMAX_DELAY. hammer.
-    - destruct PRE as (ctr & IDX & SENTRY & SENTRY_VAL & ValueValid & A0 & L_NN & MEM & A1 & A3 & Len_Nz & CtrMax &
-                        Len & CtrDist & Cycles).
+    - destruct PRE as (ctr & nxt & IDX & SENTRY & SENTRY_VAL & ValueValid & PXLH_NN & 
+            MEM & A1 & A3 & Len_Nz & CtrMax & Nxt & CtrDist & S_NN & Cycles).
         repeat step.
-        -- hammer. replace ctr with le_dist.
-            hammer.
+        -- hammer.  replace ctr with le_dist. lia.
             destruct (le_cases ctr le_dist CtrMax); try lia.
-            clear - H CtrDist IDX Len Len_Nz BC A0.
+            clear - IDX MEM Len_Nz Nxt CtrDist S_NN BC H.
             destruct IDX as (gt_node & gt_val & LeDist & LeVal & LeNextGt & GtVal & _ & Vals & _ & Lens & Sorted).
             exfalso.
-            pose proof (not_at_end_next _ _ _ _ _ Len CtrDist ltac:(lia)).
-            destruct H0 as (a0nxt & a0eq).
-            specialize (Sorted a0nxt (S ctr) (base_mem Ⓓ[base_mem Ⓓ[4 + s' R_A0]])).
-            pose proof (node_distance_next_S_len _ _ _ _ _ a0eq (distance_null_imp_well_formed _ _ _ Len) CtrDist).
-            specialize (Sorted H0).
-            enough (list_node_value base_mem a0nxt = Some (base_mem Ⓓ[base_mem Ⓓ[ 4 + s' R_A0 ]])).
-            destruct (s' R_A0).
-                contradiction.
-            specialize (Sorted H1).
-            apply N.ltb_lt in BC. lia.
-            pose proof (not_at_end_next _ _ _ _ _ Len H0 ltac:(lia)).
-            destruct H1 as (a0nxt2 & a0eq2).
-            destruct a0nxt eqn:E. inversion a0eq2.
-            unfold list_node_value. rewrite <- E in *; clear E.
-            replace a0nxt with (base_mem Ⓓ[ 4 + s' R_A0 ]). reflexivity.
-            destruct (s' R_A0). contradiction.
-                unfold list_node_next in a0eq.
-                change 4 with p.dw. remember (p.dw + N.pos p0).
-                injection a0eq. now intro.
-        -- exists (S ctr). split. assumption.
+            specialize (Sorted nxt ctr).
+            unfold list_node_next in Nxt. destruct (s' R_A4). inversion Nxt.
+            unfold p.w, p.e, p.pw, p.dw in Nxt. apply Some_inv in Nxt.
+            rewrite MEM in Nxt.
+            assert (exists v, list_node_value base_mem nxt = Some v) by admit.
+            destruct H0 as (v & H0).
+            specialize (Sorted v CtrDist H0).
+            destruct Sorted. unfold list_node_value in H0.
+            rewrite Nxt in BC. destruct nxt. inversion H0.
+            apply Some_inv in H0. unfold p.w, p.e, p.dw in H0.
+            subst v. specialize (H1 ltac:(lia)). lia.
+        -- exists (S ctr). 
+            assert (exists nxt', list_node_next base_mem nxt = Some nxt') by admit.
+            destruct H as (nxt' & H). exists nxt'.
+            split. assumption.
             destruct IDX as (gt_node & gt_val & LeDist & LeVal & LeNextGt & GtVal & GtNN & Vals & MaxVal & Lens & Sorted).
             repeat split; auto; try lia; try now rewrite <- MEM.
-            intro Contra.
-                replace sentry with (s' R_A0) in *.
-                rewrite MEM in *.
-                specialize (Sorted _ _ _ SENTRY SENTRY_VAL).
-                destruct (Nat.le_gt_cases (len - 1) le_dist). lia.
-                assert (S ctr < len)%nat by lia.
-                pose proof (at_end_lens _ _ _ _ _ L_NN Len CtrDist).
-                destruct H1; try lia.
-                destruct (s' R_A0). contradiction. change 4 with p.dw in Contra.
-                unfold list_node_next. f_equal. apply Contra.
-                pose proof (distance_last_node base_mem l (s' R_A0) ctr A0 CtrDist).
-                destruct (s' R_A0). contradiction. unfold list_node_next in H.
-                unfold p.w, p.e, p.pw, p.dw in H. rewrite Contra in H.
-                specialize (H ltac:(reflexivity)).
-                assert (S ctr = len) by eauto using node_distance_uniq.
-                subst len. simpl in SENTRY. rewrite Nat.sub_0_r in SENTRY.
-                eapply node_distance_uniq'; eauto. now rewrite <- MEM.
             destruct (le_cases ctr le_dist CtrMax). lia.
-                subst ctr.
+                subst le_dist.
                 pose proof (node_distance_uniq' _ _ _ _ _ _ LeDist CtrDist eq_refl).
                 subst le_node.
                 apply N.ltb_ge in BC.
-                (* specialize (Sorted _ _ _ LeDist ltac:(lia) LeVal). *)
-                destruct (s' R_A0). contradiction.
-                replace gt_node with (base_mem Ⓓ[4 + N.pos p]) in *.
-                destruct (base_mem Ⓓ[ 4 + N.pos p ]). contradiction.
+                destruct (s' R_A4). inversion Nxt.
+                unfold list_node_next in Nxt. apply Some_inv in Nxt.
+                unfold p.w, p.e, p.dw, p.pw in *. rewrite <- MEM, Nxt in BC.
+                destruct nxt. inversion H.
+                assert (gt_node = nxt'). {
+                    rewrite H in LeNextGt. now inversion LeNextGt.
+                } subst gt_node. inversion LeVal.
+                unfold p.w, p.e, p.dw, p.pw in *. rewrite MEM, H1 in BC.
+                specialize (Sorted nxt' (S ctr)).
+                assert (exists v, list_node_value (s' V_MEM32) nxt' = Some v) by admit.
+                destruct H0 as (v & H0).
+                specialize (Sorted v).
+                assert (node_distance base_mem pxListHead nxt' (S ctr)) by admit.
+                destruct nxt'. contradiction.
                     inversion GtVal. subst gt_val. clear - Vals BC.
-                    replace (getmem p.w p.e p.dw base_mem (N.pos p0)) with (base_mem Ⓓ[N.pos p0]) in Vals by reflexivity.
+                    unfold p.w, p.e, p.dw in *.
                     lia.
-                destruct (N.pos p). contradiction. now inversion LeNextGt.
+                unfold list_node_next in Nxt. apply Some_inv in Nxt.
+                unfold p.w, p.e, p.pw, p.dw in *. rewrite <- Nxt in *.
+                inversion LeNextGt.
             eapply node_distance_next_S_len with (dst := s' R_A0).
                 destruct (s' R_A0). contradiction. reflexivity.
             eapply distance_null_imp_well_formed. now eassumption.
